Finished refactoring of general_bf.v

examples/sbf/ConFilter.v
@@ -6,9 +6,11 @@ Open Scope Z_scope.
 
 Section ConFilter.
 
-Definition row num_slots := { r: list bool | Zlength r = num_slots }.
+Definition items (T: Type) size := { i: list T | Zlength i = size }.
 
-Definition frame num_rows num_slots := { fr: list (row num_slots) | Zlength fr = num_rows }.
+Definition row num_slots := items bool num_slots.
+
+Definition frame num_rows num_slots := items (row num_slots) num_rows.
 
 Program Definition row_insert {num_slots} (r : row num_slots) (i : Z) : row num_slots :=
   upd_Znth i r true.
@@ -17,10 +19,15 @@ Next Obligation.
   destruct r. easy.
 Qed.
 
-Definition items size := { i: list Z | Zlength i = size }.
+Lemma row_insert_comm {num_slots}: forall (r: row num_slots) x y,
+    row_insert (row_insert r x) y = row_insert (row_insert r y) x.
+Proof.
+  intros. destruct r as [r ?H]. unfold row_insert. simpl.
+  apply subset_eq_compat. list_solve.
+Qed.
 
 Program Definition frame_insert {num_rows num_slots} (f : frame num_rows num_slots)
-  (is : items num_rows) : frame num_rows num_slots := map2 row_insert f is.
+  (is : items Z num_rows) : frame num_rows num_slots := map2 row_insert f is.
 Next Obligation.
   rewrite Zlength_map2. destruct is, f. simpl. lia.
 Qed.
@@ -38,13 +45,19 @@ Next Obligation.
 Qed.
 
 Program Definition frame_clear {num_rows num_slots} (f : frame num_rows num_slots)
-  (is : items num_rows) : frame num_rows num_slots:= map2 row_clear f is.
+  (is : items Z num_rows) : frame num_rows num_slots:= map2 row_clear f is.
 Next Obligation.
   rewrite Zlength_map2. destruct is, f. simpl. lia.
 Qed.
 
 Program Definition row_query {num_slots} (r : row num_slots) (i : Z) : bool :=
   Znth i r.
+
+Lemma row_query_insert_true {num_slots}: forall (r: row num_slots) z,
+    0 <= z < num_slots -> row_query (row_insert r z) z = true.
+Proof.
+  intros. destruct r as [r ?H]. unfold row_query, row_insert. simpl. list_solve.
+Qed.
 
 Program Definition frame_query {num_rows num_slots} (f : frame num_rows num_slots)
   (is : list Z) : bool :=
