examples/sbf/Utils.v
@@ -17,6 +17,12 @@ Definition map2 {A B C} (f : A -> B -> C) (al : list A) (bl : list B) : list C :
 Lemma fold_andb_false: forall l, fold_left andb l false = false.
 Proof. induction l; simpl; intros; auto. Qed.
 
+Lemma fold_andb_cons: forall l b, fold_andb (b :: l) = (b && fold_andb l)%bool.
+Proof.
+  intros. unfold fold_andb. simpl. destruct b; simpl; auto.
+  apply fold_andb_false.
+Qed.
+
 Lemma map2_cons {A B C}: forall (f : A -> B -> C) a al b bl,
     map2 f (a :: al) (b :: bl) = f a b :: map2 f al bl.
 Proof. intros. unfold map2. simpl. auto. Qed.
